As $N\to\infty$,
$$
\Pr(X=i)=2^{-i}\quad (i\ge 1),\qquad F(m)=\Pr(X\le m)=\sum_{i=1}^m 2^{-i}=1-2^{-m}.
$$
For (J) i.i.d. turns,
$$
\Pr(M\le m)=F(m)^J=(1-2^{-m})^J.
$$
Using the tail-sum formula,
$$
\mathbb E[M]=\sum_{m\ge 1}\Pr(M\ge m)
= \sum_{m\ge 1}\Bigl(1-\Pr(M\le m-1)\Bigr)
= \sum_{k\ge 0}\Bigl(1-(1-2^{-k})^J\Bigr),
$$
where $k=m-1$.

Expand with the binomial theorem:
$$
1-(1-2^{-k})^J
= \sum_{t=1}^J (-1)^{t+1}\binom{J}{t}2^{-kt}.
$$
Swap sums (all terms are nonnegative after the first expression, so the manipulation is valid):
$$
\mathbb E[M]
=\sum_{t=1}^J (-1)^{t+1}\binom{J}{t}\sum_{k\ge 0}2^{-kt}
=\sum_{t=1}^J (-1)^{t+1}\binom{J}{t}\cdot \frac{1}{1-2^{-t}}
=\sum_{t=1}^J (-1)^{t+1}\binom{J}{t}\cdot \frac{2^{t}}{2^{t}-1}.
$$

So for $J=696969$,
$$
\mathbb E[M]\equiv \sum_{t=1}^{696969} (-1)^{t+1}\binom{696969}{t} 2^{t} (2^{t}-1)^{-1}\pmod{10^9+7}.
$$

Evaluating that sum modulo (10^9+7) gives:

$$
\boxed{123019395}.
$$
